used QC to test the source examples

I2SFI/CompilerIntegrationTests.v
@@ -8,7 +8,9 @@ Require Import Coq.Strings.String.
 Require Import CompCert.Events.
 
 Require Import Source.Language.
-Require Import Source.Examples.
+Require Import Source.Examples.Factorial.
+Require Import Source.Examples.Identity.
+Require Import Source.Examples.Increment.
 Require Import S2I.Compiler.
 Require Import I2SFI.Compiler.
 Require Import TargetSFI.EitherMonad.
@@ -20,6 +22,11 @@ Require Import Common.Maps.
 
 Import MonadNotations.
 Open Scope monad_scope.
+
+From QuickChick Require Import QuickChick.
+Import QcDefaultNotation. Import QcNotation. Open Scope qc_scope.
+Import GenLow GenHigh.
+(* Suppress some annoying warnings: *)
 
 Open Scope positive_scope.
 Definition increment : Source.program := {|
@@ -44,16 +51,25 @@ Close Scope positive_scope.
 
 Definition test (sp : Source.program) : @Either sfi_program :=
   match S2I.Compiler.compile_program sp with
-  | None => Left "S2I compiler failed"
+  | None => TargetSFI.EitherMonad.Left "S2I compiler failed"
   | Some ip => compile_program ip
   end.
 
 
 Example test_increment :
   exists (tp : sfi_program),
-    test increment = Right tp.
+    test increment = TargetSFI.EitherMonad.Right tp.
 Proof.
   compute. eauto. Qed.
+
+(* (* this doesn't end Need to figure out TODO *) *)
+(* Example test_identity : *)
+(*   exists (ip : Intermediate.program) (tp : sfi_program), *)
+(*     S2I.Compiler.compile_program identity = Some ip /\ *)
+(*     I2SFI.Compiler.compile_program ip = Right tp. *)
+(* Proof. *)
+(*   compute. eauto. Qed. *)
+
 
 (* (* this doesn't end Need to figure out TODO *) *)
 (* Example test_factorial : *)
@@ -63,3 +79,32 @@ Proof.
 (* Proof. *)
 (*   compute. eauto. Qed. *)
 
+Instance show_sp : Show Source.program :=
+  {|
+    show := fun _ => Coq.Strings.String.EmptyString
+  |}.
+
+Definition genSourceProgram : G  Source.program :=
+  elements identity [identity; factorial;
+                       Source.Examples.Increment.increment].
+
+
+Definition integration_pbt : Checker :=
+  forAll genSourceProgram
+         ( fun sp =>
+             match S2I.Compiler.compile_program sp with
+             | None => whenFail "Source program does not compile" false
+             | Some ip =>
+               match I2SFI.Compiler.compile_program ip with
+               | TargetSFI.EitherMonad.Left msg =>
+                  whenFail ("Compilation error: " ++ msg) false
+               | TargetSFI.EitherMonad.Right p =>
+                 match CS.eval_program (5000%nat) p (RiscMachine.RegisterFile.reset_all) with
+                 | TargetSFI.EitherMonad.Left msg => whenFail msg false
+                 | TargetSFI.EitherMonad.Right (t,(mem,_,regs)) => checker true
+                 end
+               end
+             end
+         ).
+
+QuickChick integration_pbt.
